case_study/RiscvPmp/BlockVer/Spec.v
@@ -422,13 +422,6 @@ Module RiscvPmpBlockVerifSpec <: Specification RiscvPmpBase RiscvPmpProgram Risc
        lemma_postcondition   := ⊤;
     |}.
 
-  Definition lemma_update_pmp_entries : SepLemma update_pmp_entries :=
-    {| lemma_logic_variables := ctx.nil;
-       lemma_patterns        := env.nil;
-       lemma_precondition    := ⊤;
-       lemma_postcondition   := ⊤;
-    |}.
-
   Definition LEnv : LemmaEnv :=
     fun Δ l =>
       match l with
@@ -436,7 +429,7 @@ Module RiscvPmpBlockVerifSpec <: Specification RiscvPmpBase RiscvPmpProgram Risc
       | close_gprs                         => lemma_close_gprs
       | open_pmp_entries                   => lemma_machine_unlocked_open_pmp_entries
       | close_pmp_entries                  => lemma_machine_unlocked_close_pmp_entries
-      | update_pmp_entries                 => lemma_update_pmp_entries
+      | update_pmp_entries                 => lemma_machine_unlocked_update_pmp_entries
       | extract_pmp_ptsto                  => lemma_extract_pmp_ptsto
       | return_pmp_ptsto                   => lemma_return_pmp_ptsto
       end.
@@ -874,6 +867,15 @@ Module RiscvPmpIrisInstanceWithContracts.
     now iPureIntro.
   Qed.
 
+  Lemma machine_unlocked_update_pmp_entries_sound `{sailGS Σ} :
+    ValidLemma RiscvPmpSpecification.lemma_machine_unlocked_update_pmp_entries.
+  Proof.
+    intros ι; destruct_syminstance ι; cbn.
+    iIntros "(? & ? & ? & ? & %Hunlocked0 & %Hunlocked1 & ?)".
+    iFrame.
+    now iPureIntro.
+  Qed.
+
   Lemma in_liveAddrs_split : forall (addr : Addr),
       (minAddr <= addr)%Z ->
       (addr <= maxAddr)%Z ->
@@ -931,6 +933,7 @@ Module RiscvPmpIrisInstanceWithContracts.
     intros Δ []; intros ι; destruct_syminstance ι; try now iIntros "_".
     - apply machine_unlocked_open_pmp_entries_sound.
     - apply machine_unlocked_close_pmp_entries_sound.
+    - apply machine_unlocked_update_pmp_entries_sound.
     - apply extract_pmp_ptsto_sound.
     - apply return_pmp_ptsto_sound.
   Qed.
